coq/cttwc/disequality.v
@@ -4,8 +4,10 @@ Admitted.
 
 
 (* bool = nat type-checks since bool and nat have same sort Set                 *)
+(*
 Check bool.
 Check nat.
+*)
 
 (* This is going to be true for bool but not for nat.                          *)
 Definition P1 (X:Type) : Prop := forall (x y z:X), x = y \/ x = z \/ y = z.
@@ -38,9 +40,11 @@ Proof.
     intros H. apply L4. rewrite <- H. apply L2.
 Qed.
 
+(*
 Check True. (* Prop *)
 Check unit. (* Set  *)
 Check bool. (* Set  *)
+*)
 
 (* Different sorts but still seems ok                                           *)
 Definition L6 : bool <> True.
@@ -50,4 +54,56 @@ Admitted.
 Definition L7 : bool <> unit.
 Proof.
 Admitted.
+
+(* true for unit but not for bool.                                              *)
+Definition P2 (X:Type) : Prop := forall (x y:X), x = y.
+
+Definition L8 : P2 unit.
+Proof.
+    intros x y. destruct x; destruct y. reflexivity.
+Qed.
+
+Definition L9 : P2 unit.
+Proof.
+refine (
+    fun (x y:unit) => 
+        match x, y with
+        | tt, tt    => eq_refl tt
+        end
+). 
+Qed.
+
+Definition L10 : true <> false.
+Proof.
+    intros H. inversion H.
+Qed.
+
+
+Definition L11 : ~ P2 bool.
+Proof.
+    unfold P2. intros H. apply L10. apply H.
+Qed.
+
+Definition L12 : bool <> unit.
+Proof.
+    intros H. apply L11. rewrite H. apply L9.
+Qed.
+
+Definition L13 : ~ ( (true,true) = (true,false) 
+                  \/ (true,true) = (false,false) 
+                  \/ (true, false) = (false, false)).
+Proof. intros [H|[H|H]]; inversion H. Qed.
+
+
+Open Scope type_scope.
+
+Definition L14 : ~ P1 (bool * bool).
+Proof.
+    unfold P1. intros H. apply L13. apply H.
+Qed.
+
+Definition L15 : bool * bool <> bool.
+Proof.
+    intros H. apply L14. rewrite H. apply L2.
+Qed.
 
