coq/set/Normal/Sort.v
@@ -4,4 +4,59 @@ Require Import Core.Set.
 
 Require Import Normal.Leq.
 Require Import Normal.Equiv.
+Require Import Normal.Insert.
 Require Import Normal.InListOf.
+
+(* Sorting elements of set as per syntax.                                       *)
+Definition sort (x:set) : set := fromList (Sort.sort (toList x)).
+
+Definition Sorted (x:set) : Prop := Sort.Sorted (toList x).
+
+Lemma sortEquiv : forall (x:set), Equiv x (sort x).
+Proof.
+    intros x. unfold Equiv, sort. rewrite toListFromList.
+    apply Sort.sortEquiv.
+Qed.
+
+Lemma sortInListOfIff : forall (x xs:set), 
+    inListOf x xs <-> inListOf x (sort xs).
+Proof.
+    intros x xs. unfold inListOf, sort. rewrite toListFromList.
+    apply Sort.sortInIff.
+Qed.
+
+Lemma insertSorted : forall (x xs:set), 
+    Sorted xs -> Sorted (insert x xs).
+Proof.
+    intros x xs. rewrite insertCorrect. unfold Sorted, insertAsList.
+    rewrite toListFromList. apply Sort.insertSorted.
+Qed.
+
+Lemma sortSorted : forall (x:set), Sorted (sort x).
+Proof.
+    intros x. unfold Sorted, sort. rewrite toListFromList. 
+    apply Sort.sortSorted.
+Qed.
+
+Lemma sortedConsInListOfLeq : forall (x y xs:set),
+    Sorted (Cons x xs) -> inListOf y xs -> leq y x.
+Proof.
+    intros x y xs. unfold Sorted, inListOf. apply Sort.sortedConsInLeq.
+Qed.
+
+Lemma sortedCons : forall (x xs:set),
+    (forall (z:set), inListOf z xs -> leq z x) -> 
+    Sorted xs -> 
+    Sorted (Cons x xs).
+Proof.
+    intros x xs. unfold inListOf, Sorted. intros H1 H2.
+    apply (Sort.sortedCons set _ x (toList xs)); assumption.
+Qed.
+
+Lemma sortSame : forall (x:set), Sorted x -> sort x = x.
+Proof.
+    intros x. unfold Sorted, sort. intros H. 
+    rewrite <- (fromListToList x) at 2. rewrite Sort.sortSame.
+    - reflexivity.
+    - assumption.
+Qed.
