coq/cttwc/funspec.v
@@ -1,0 +1,38 @@
+Definition Add (f:nat -> nat -> nat) : Prop 
+    := (forall (y:nat), f 0 y = y) 
+    /\ (forall (x y:nat), f (S x) y = S (f x y)).
+
+(* uniqueness up to functional extensionality                                   *)
+Definition L1 : forall (f g:nat -> nat -> nat),
+    Add f -> Add g -> forall (x y:nat), f x y = g x y.
+Proof.
+    intros f g [H1 H2] [H3 H4]. induction x as [|x IH]; intros y.
+    - rewrite H1, H3. reflexivity.
+    - rewrite H2, H4, IH. reflexivity.
+Qed.
+
+(* existence                                                                    *)
+Definition L2 : Add (fun (x y:nat) => x + y).
+Proof.
+    unfold Add. split; intros y; reflexivity.
+Qed.
+
+
+
+Definition FunExt : Prop := forall (a b:Type) (f g:a -> b), 
+    (forall (x:a), f x = g x) -> f = g.
+
+
+Definition Ack (f:nat -> nat -> nat) : Prop 
+    := (forall (y:nat), f 0 y = S y)
+    /\ (forall (x:nat), f (S x) 0 = f x 1)
+    /\ (forall (x y:nat), f (S x) (S y) = f x (f (S x) y)).
+
+(* uniqueness up to functional extensionality                                   *)
+Definition L3 : forall (f g:nat -> nat -> nat),
+    Ack f -> Ack g -> forall (x y:nat), f x y = g x y.
+Proof.
+    intros f g [H1 [H2 H3]] [H4 [H5 H6]]. induction x as [|x IH].
+    - intros y. rewrite H1, H4. reflexivity.
+    - 
+Show.
