lean/funext.lean
@@ -1,0 +1,11 @@
+universes u v
+
+axiom funext2 : ∀ {α : Sort u} {β : α → Sort v} {f g : ∀ (x:α), β x},
+  (∀ (x:α), f x = g x) → f = g
+
+--#check @funext2
+--#check @funext
+
+
+lemma L1 : Prop = Sort 0 := rfl
+lemma L2 : Type u = Sort (u + 1) := rfl
