lean/propext.lean
@@ -1,5 +1,8 @@
 axiom propext2 {p q : Prop} : (p ↔ q) → p = q
 
+--#check @propext2
+--#check @propext
+
 variables p q r s t : Prop
 variable P : Prop -> Prop
 
@@ -17,3 +20,12 @@ begin
 end
 
 -- L2 is equivalent to propext
+lemma L3 :
+  (∀ (p q : Prop), (p ↔ q) → p = q)
+  ↔
+  (∀ (P : Prop → Prop) (p q:Prop), (p ↔ q) → (P p → P q)) :=
+begin
+  split,
+    {intros H1 P p q H2 H3, rewrite ← (H1 p q H2), assumption},
+    {intros H1 p q H2, apply H1 (λ z, p = z) p q H2 rfl}
+end
